## Medium Logic Exercises

### CNF I

What is the first step in converting (p ∨ q) ∧ (p ∧ r) to its CNF?

### CNF II

Take a sheet of paper and find out the CNFs of the sentences: 

- ¬(A ∨ B) ⇔ C
- (p ⇒ q) ⇒ r 
- p ⇔ q 





[View Solutions for Medium Logic](https://github.com/UMdecisionsupport/DecisionSupport2023/blob/main/Logic/Solutions/Medium_Solutions.md)

[Move back to Beginner Logic Exercises](https://github.com/UMdecisionsupport/DecisionSupport2023/blob/main/Logic/Beginner.md)

[Move forward to Advanced Logic Exercises](https://github.com/UMdecisionsupport/DecisionSupport2023/blob/main/Logic/Advanced.md)
